softwarefoundations/vol2_plf/HoareAsLogic.v
@@ -1,0 +1,273 @@
+Set Warnings "-deprecated-hint-without-locality,-deprecated-hint-without-locality".
+From PLF Require Import Maps.
+From PLF Require Import Hoare.
+Hint Constructors ceval : core.
+
+
+Inductive derivable : Assertion -> com -> Assertion -> Type :=
+  | H_Skip : forall P,
+      derivable P <{skip}> P
+  | H_Asgn : forall Q V a,
+      derivable (Q [V |-> a]) <{V := a}> Q
+  | H_Seq : forall P c Q d R,
+      derivable P c Q -> derivable Q d R -> derivable P <{c;d}> R
+  | H_If : forall P Q (b: bexp) c1 c2,
+    derivable (P /\  b) c1 Q ->
+    derivable (P /\ ~b) c2 Q ->
+    derivable P <{if b then c1 else c2 end}> Q
+  | H_While : forall P (b: bexp) c,
+    derivable (P /\ b) c P ->
+    derivable P <{while b do c end}> (P /\ ~b)
+  | H_Consequence : forall (P Q P' Q' : Assertion) c,
+    derivable P' c Q' ->
+    (P ->> P') ->
+    (Q' ->> Q) ->
+    derivable P c Q.
+
+Lemma H_Consequence_pre : forall (P Q P': Assertion) c,
+    derivable P' c Q ->
+    (P ->> P') ->
+    derivable P c Q.
+Proof. eauto using H_Consequence. Qed.
+
+Lemma H_Consequence_post : forall (P Q Q' : Assertion) c,
+    derivable P c Q' ->
+    (Q' ->> Q) ->
+    derivable P c Q.
+Proof. eauto using H_Consequence. Qed.
+
+Example sample_proof :
+  derivable
+    ((assert (X = 3)) [X |-> X + 2] [X |-> X + 1])
+    <{ X := X + 1; X := X + 2}>
+    (assert (X = 3)).
+Proof.
+  eapply H_Seq.
+  - apply H_Asgn.
+  - apply H_Asgn.
+Qed.
+
+Theorem provable_true_post : forall c P,
+    derivable P c True.
+Proof.
+  intro c.
+  induction c; intro P.
+  - eapply H_Consequence_post.
+    eapply (H_Skip).
+    auto.
+  - eapply H_Consequence_pre.
+    eapply (H_Asgn).
+    auto.
+  - eapply (H_Seq).
+    apply IHc1.
+    apply IHc2.
+  - apply H_If.
+    apply IHc1.
+    apply IHc2.
+  - eapply H_Consequence.
+    eapply H_While.
+    apply IHc.
+    auto. auto.
+Qed.
+
+
+Lemma false_assrt: forall Q, False ->> Q.
+Proof. intros Q st F. simpl in F. destruct F. Qed.
+
+Theorem provable_false_pre : forall c Q,
+    derivable False c Q.
+Proof.
+  intro c.
+  induction c; intro Q.
+  - eapply H_Consequence_pre.
+    eapply (H_Skip).
+    apply false_assrt.
+  - eapply H_Consequence_pre.
+    eapply (H_Asgn).
+    apply false_assrt.
+  - eapply (H_Seq).
+    apply IHc1.
+    apply IHc2.
+  - eapply H_If.
+    + eapply H_Consequence_pre.
+      apply IHc1. simpl.
+      intros st [F _]. apply F.
+    + eapply H_Consequence_pre.
+      apply IHc2. simpl.
+      intros st [F _]. apply F.
+  - eapply H_Consequence.
+    + eapply H_While.
+      eapply H_Consequence_pre.
+      eapply IHc.
+      intros st [F _]. apply F.
+    + apply false_assrt.
+    + simpl. intros st [F _]. destruct F.
+Qed.
+
+
+Theorem hoare_sound : forall P c Q,
+  derivable P c Q -> {{P}} c {{Q}}.
+Proof.
+  intros P c Q Hder.
+  induction Hder; intros st st' com Hp.
+  - inversion com; subst. assumption.
+  - inversion com; subst. unfold assn_sub in Hp. assumption.
+  - inversion com; subst.
+    eapply IHHder2. apply H4.
+    eapply IHHder1. apply H1.
+    apply Hp.
+  - inversion com; subst.
+    + (* if true *)
+      eapply IHHder1. apply H5.
+      split. apply Hp. apply H4.
+    + (* if false *)
+      eapply IHHder2. apply H5.
+      split. apply Hp. simpl. intro Contra. congruence.
+  - remember <{ while b do c end }> as k eqn:Ek.
+    induction com; try (discriminate Ek).
+    + injection Ek as Ek1 Ek2. subst. split.
+      * assumption.
+      * intro Contra. congruence.
+    + injection Ek as Ek1 Ek2. subst.
+      apply IHcom2; try reflexivity.
+      eapply IHHder.
+      apply com1.
+      split.
+      * assumption.
+      * apply H.
+  - apply a0.
+    eapply IHHder.
+    apply com.
+    apply a.
+    assumption.
+Qed.
+
+
+
+(* Weakest precondifiton for Q *)
+Definition wp (c:com) (Q:Assertion) : Assertion :=
+  fun s => forall s', s =[ c ]=> s' -> Q s'.
+Hint Unfold wp : core.
+
+Theorem wp_is_precondition : forall c Q,
+  {{wp c Q}} c {{Q}}.
+Proof. intros c Q st st' com. unfold wp. intro H. auto. Qed.
+
+Theorem wp_is_weakest : forall c Q P',
+    {{P'}} c {{Q}} -> P' ->> (wp c Q).
+Proof. eauto. Qed.
+
+
+Lemma wp_seq : forall P Q c1 c2,
+    derivable P c1 (wp c2 Q) -> derivable (wp c2 Q) c2 Q -> derivable P <{c1; c2}> Q.
+Proof.
+  intros P Q c1 c2 H1 H2.
+  eapply H_Seq.
+  apply H1.
+  apply H2.
+Qed.
+
+Lemma wp_invariant : forall b c Q,
+    hoare_triple (wp <{while b do c end}> Q /\ b) c (wp <{while b do c end}> Q).
+Proof.
+  intros b c Q st st' com [H1 H2].
+  unfold wp in *.
+  intros s' comWhile.
+  apply H1.
+  eapply E_WhileTrue.
+  - apply H2.
+  - apply com.
+  - apply comWhile.
+Qed.
+
+(*
+Lemma split_seq: forall P Q c1 c2, 
+  {{P}} c1; c2 {{Q}} -> {{wp c2 Q}} c2 {{Q}} /\ {{P}} c1 {{wp c2 Q}}.
+Proof.
+  intros P Q c1 c2 H.
+  unfold hoare_triple in H.
+  split.
+  - intros st' st'' comC2 Hwp. 
+    eapply (H).
+    eapply E_Seq.
+*)
+
+Theorem hoare_complete: forall P c Q,
+  {{P}} c {{Q}} -> derivable P c Q.
+Proof.
+  intros P c. generalize dependent P.
+  induction c; intros P Q HT.
+  - (* skip *)
+    eapply H_Consequence_post.
+    apply H_Skip.
+    intros st Hpst.
+    unfold hoare_triple in HT.
+    apply (HT st st).
+    + apply E_Skip.
+    + assumption.
+  - (* assign *)
+    eapply H_Consequence_pre.
+    apply H_Asgn.
+    intros st Hpst.
+    unfold hoare_triple in HT.
+    apply (HT st).
+    + apply E_Asgn.
+      reflexivity.
+    + assumption.
+  - (* seq *)
+    apply wp_seq.
+    + apply IHc1.
+      unfold hoare_triple in HT.
+      intros st st' comC1 Hpst. unfold wp.
+      intros s' comC2.
+      eapply HT.
+      eapply E_Seq.
+      apply comC1.
+      apply comC2.
+      apply Hpst.
+    + apply IHc2.
+      unfold hoare_triple in HT.
+      intros st st' comC2 Hwp.
+      apply Hwp.
+      apply comC2.
+  - (* if *)
+    apply H_If.
+    + (* true *)
+      apply IHc1.
+      intros st st' comC1 [Hpst Hb].
+      eapply HT.
+      apply E_IfTrue.
+      apply Hb.
+      apply comC1.
+      apply Hpst.
+    + (* false *)
+      apply IHc2.
+      intros st st' comC1 [Hpst Hnotb].
+      eapply HT.
+      apply E_IfFalse.
+      assert (G: beval st b = false). {
+        destruct (beval st b) eqn:Hb.
+        * exfalso. apply Hnotb. apply Hb.
+        * reflexivity.
+      }
+      apply G.
+      apply comC1.
+      apply Hpst.
+  - (* while *)
+    eapply H_Consequence.
+    + eapply H_While.
+      apply IHc.
+      apply wp_invariant.
+    + apply wp_is_weakest.
+      apply HT.
+    + intros st [H1 H2].
+      apply H1.
+      apply E_WhileFalse.
+      assert (G: beval st b = false). {
+        destruct (beval st b) eqn:Hb.
+        * exfalso. apply H2. apply Hb.
+        * reflexivity.
+      }
+      apply G.
+Qed.
+
